writing/presentation.md
@@ -1,0 +1,126 @@
+### Amortized Analysis
+
+In order to analyse the cost of a sequence of operations on a given data structure we use
+the potential method. Inspired by the concept of potential energy in physics, the idea is
+to assign a function $\Phi(D)$ that maps the data structure $D$ to the positive integers.
+Operations on $D$ may cause it to gain or lose potential. The amortized cost
+$A(op(D))$ of an operation $op(D)$ is defined as its actual cost $K(op(D))$ and the
+difference in potentials before and after its evaluation, $A(op(D)) = K(op(D)) + \Phi(op(D)) - \Phi(D)$
+
+### Amortized Analysis
+
+The sum of the amortized costs taken over a sequence of operations plus the potential
+of the initial data structure then furnishes an upper bound for the actual cost
+of that sequence
+
+$$ \Phi(D_0) + \sum_{1 \leq i \leq n}{A(op(D_i))} = \Phi(D_0) + \sum_{1 \leq i \leq n}{K(op(D_i)) + \Phi(D_i) - \Phi(D_{i-1})} $$
+$$ = \Phi(D_n) + \sum_{1 \leq i \leq n}{K(op(D_i))} \geq \sum_{1 \leq i \leq n}{K(op(D_i))} $$
+
+
+### Example
+
+The classical example for the potential method of amortized analysis is the functional queue,
+implemented as two lists $L_{in}$ and $L_{out}$ acting as stacks.
+Trying to determine the number of list operations required to perform a sequence of
+*enqueue* and *dequeue* operations we find a problem: the cost of a *dequeue* is not constant.
+Whenever $L_{out}$ is empty, we transfer elements from $L_{in}$ before removing an element.
+
+To aid our analysis we introduce the potential $\Phi(L_{in}, L_{out}) = 2\cdot|L_{in}|$.
+The amortized cost of *enqueue* is then $A(enqueue) = 3$, one to pay for the attachment
+to $L_{in}$ and two to pay for the increase in potential.
+The amortized cost of *dequeue* is $A(dequeue) = 1$, to see why consider the two cases:
+if $L_{out}$ is not empty then we just detach the first element of $L_{out}$ and the
+potential is unchanged; if $L_{out}$ is not empty then we have to move the elements in $L_{in}$ to
+$L_{out}$, the actual cost is then $2 \cdot |L_{in}|$ but because $L_{in}$ is now empty
+$2 \cdot |L_{in}|$ is exactly the decrease in potential.
+So the amortized cost is $1$.
+
+### Example
+
+Finally we can conclude that given a queue with $|L_{in}|$ equal to $k$,
+the number of list operations in a sequence of $m$  $enqueue$ and $n$  $dequeue$
+operations is less than $3 \cdot m + n + 2\cdot k$
+
+
+### Examples
+
+~~~
+type nat =
+	| O
+	| S of nat
+
+let rec add n m =
+	match n with
+	| O -> m
+	| S n1 -> (add n1 (S m))
+
+let rec mult n m =
+	match n with
+	| O -> O
+	| S n1 -> add m (mult n1 m)
+
+let rec square n = mult n n
+~~~
+
+### Results
+
+~~~
+== add :
+
+  [nat; nat] -> nat
+
+  Non-zero annotations of the argument:
+		8  <--  ([S(*)], [])
+		3  <--  ([], [])
+
+  Non-zero annotations of result:
+
+  Simplified bound:
+	3 + 8*M
+   where
+	M is the number of S-nodes of the
+	1st component of the argument
+~~~
+
+### Results
+
+~~~
+== mult :
+
+  [nat; nat] -> nat
+
+  Non-zero annotations of the argument:
+		8  <--  ([S(*)], [S(*)])
+		12  <--  ([S(*)], [])
+		3  <--  ([], [])
+
+  Non-zero annotations of result:
+
+  Simplified bound:
+	3 + 8*L*M + 12*M
+   where
+	L is the number of S-nodes of the
+	2nd component of the argument
+	M is the number of S-nodes of the
+	1st component of the argument
+~~~
+
+### Results
+
+~~~
+== square :
+
+  nat -> nat
+
+  Non-zero annotations of the argument:
+		16  <--  [S(*); S(*)]
+		20  <--  [S(*)]
+		7  <--  []
+
+  Non-zero annotations of result:
+
+  Simplified bound:
+	7 + 12*M + 8*M^2
+   where
+	M is the number of S-nodes of the argument
+~~~
